# The univalence axiom

<pre class="Agda"><a id="33" class="Symbol">{-#</a> <a id="37" class="Keyword">OPTIONS</a> <a id="45" class="Pragma">--without-K</a> <a id="57" class="Pragma">--exact-split</a> <a id="71" class="Symbol">#-}</a>

<a id="76" class="Keyword">module</a> <a id="83" href="foundation-core.univalence.html" class="Module">foundation-core.univalence</a> <a id="110" class="Keyword">where</a>

<a id="117" class="Keyword">open</a> <a id="122" class="Keyword">import</a> <a id="129" href="foundation-core.contractible-types.html" class="Module">foundation-core.contractible-types</a> <a id="164" class="Keyword">using</a> <a id="170" class="Symbol">(</a><a id="171" href="foundation-core.contractible-types.html#993" class="Function">is-contr</a><a id="179" class="Symbol">)</a>
<a id="181" class="Keyword">open</a> <a id="186" class="Keyword">import</a> <a id="193" href="foundation-core.dependent-pair-types.html" class="Module">foundation-core.dependent-pair-types</a> <a id="230" class="Keyword">using</a> <a id="236" class="Symbol">(</a><a id="237" href="foundation-core.dependent-pair-types.html#502" class="Record">Σ</a><a id="238" class="Symbol">;</a> <a id="240" href="foundation-core.dependent-pair-types.html#575" class="InductiveConstructor">pair</a><a id="244" class="Symbol">;</a> <a id="246" href="foundation-core.dependent-pair-types.html#592" class="Field">pr1</a><a id="249" class="Symbol">;</a> <a id="251" href="foundation-core.dependent-pair-types.html#604" class="Field">pr2</a><a id="254" class="Symbol">)</a>
<a id="256" class="Keyword">open</a> <a id="261" class="Keyword">import</a> <a id="268" href="foundation-core.equivalences.html" class="Module">foundation-core.equivalences</a> <a id="297" class="Keyword">using</a>
  <a id="305" class="Symbol">(</a> <a id="307" href="foundation-core.equivalences.html#1608" class="Function Operator">_≃_</a><a id="310" class="Symbol">;</a> <a id="312" href="foundation-core.equivalences.html#2481" class="Function">id-equiv</a><a id="320" class="Symbol">;</a> <a id="322" href="foundation-core.equivalences.html#1543" class="Function">is-equiv</a><a id="330" class="Symbol">;</a> <a id="332" href="foundation-core.equivalences.html#1808" class="Function">map-equiv</a><a id="341" class="Symbol">)</a>
<a id="343" class="Keyword">open</a> <a id="348" class="Keyword">import</a> <a id="355" href="foundation-core.fundamental-theorem-of-identity-types.html" class="Module">foundation-core.fundamental-theorem-of-identity-types</a> <a id="409" class="Keyword">using</a>
  <a id="417" class="Symbol">(</a> <a id="419" href="foundation-core.fundamental-theorem-of-identity-types.html#1891" class="Function">fundamental-theorem-id</a><a id="441" class="Symbol">;</a> <a id="443" href="foundation-core.fundamental-theorem-of-identity-types.html#2162" class="Function">fundamental-theorem-id&#39;</a><a id="466" class="Symbol">)</a>
<a id="468" class="Keyword">open</a> <a id="473" class="Keyword">import</a> <a id="480" href="foundation-core.homotopies.html" class="Module">foundation-core.homotopies</a> <a id="507" class="Keyword">using</a> <a id="513" class="Symbol">(</a><a id="514" href="foundation-core.homotopies.html#614" class="Function Operator">_~_</a><a id="517" class="Symbol">;</a> <a id="519" href="foundation-core.homotopies.html#728" class="Function">refl-htpy</a><a id="528" class="Symbol">)</a>
<a id="530" class="Keyword">open</a> <a id="535" class="Keyword">import</a> <a id="542" href="foundation-core.identity-types.html" class="Module">foundation-core.identity-types</a> <a id="573" class="Keyword">using</a> <a id="579" class="Symbol">(</a><a id="580" href="foundation-core.identity-types.html#1852" class="Function Operator">_＝_</a><a id="583" class="Symbol">;</a> <a id="585" href="foundation-core.identity-types.html#1807" class="InductiveConstructor">refl</a><a id="589" class="Symbol">;</a> <a id="591" href="foundation-core.identity-types.html#3990" class="Function">ap</a><a id="593" class="Symbol">;</a> <a id="595" href="foundation-core.identity-types.html#5689" class="Function">tr</a><a id="597" class="Symbol">)</a>
<a id="599" class="Keyword">open</a> <a id="604" class="Keyword">import</a> <a id="611" href="foundation-core.universe-levels.html" class="Module">foundation-core.universe-levels</a> <a id="643" class="Keyword">using</a> <a id="649" class="Symbol">(</a><a id="650" href="Agda.Primitive.html#597" class="Postulate">Level</a><a id="655" class="Symbol">;</a> <a id="657" href="foundation-core.universe-levels.html#222" class="Primitive">UU</a><a id="659" class="Symbol">;</a> <a id="661" href="Agda.Primitive.html#780" class="Primitive">lsuc</a><a id="665" class="Symbol">)</a>
</pre>
## Idea

The univalence axiom characterizes the identity types of universes. It asserts that the map `Id A B → A ≃ B` is an equivalence.

## Definition

<pre class="Agda"><a id="equiv-eq"></a><a id="833" href="foundation-core.univalence.html#833" class="Function">equiv-eq</a> <a id="842" class="Symbol">:</a> <a id="844" class="Symbol">{</a><a id="845" href="foundation-core.univalence.html#845" class="Bound">i</a> <a id="847" class="Symbol">:</a> <a id="849" href="Agda.Primitive.html#597" class="Postulate">Level</a><a id="854" class="Symbol">}</a> <a id="856" class="Symbol">{</a><a id="857" href="foundation-core.univalence.html#857" class="Bound">A</a> <a id="859" class="Symbol">:</a> <a id="861" href="foundation-core.universe-levels.html#222" class="Primitive">UU</a> <a id="864" href="foundation-core.univalence.html#845" class="Bound">i</a><a id="865" class="Symbol">}</a> <a id="867" class="Symbol">{</a><a id="868" href="foundation-core.univalence.html#868" class="Bound">B</a> <a id="870" class="Symbol">:</a> <a id="872" href="foundation-core.universe-levels.html#222" class="Primitive">UU</a> <a id="875" href="foundation-core.univalence.html#845" class="Bound">i</a><a id="876" class="Symbol">}</a> <a id="878" class="Symbol">→</a> <a id="880" class="Symbol">(</a><a id="881" href="foundation-core.univalence.html#857" class="Bound">A</a> <a id="883" href="foundation-core.identity-types.html#1852" class="Function Operator">＝</a> <a id="885" href="foundation-core.univalence.html#868" class="Bound">B</a><a id="886" class="Symbol">)</a> <a id="888" class="Symbol">→</a> <a id="890" href="foundation-core.univalence.html#857" class="Bound">A</a> <a id="892" href="foundation-core.equivalences.html#1608" class="Function Operator">≃</a> <a id="894" href="foundation-core.univalence.html#868" class="Bound">B</a>
<a id="896" href="foundation-core.univalence.html#833" class="Function">equiv-eq</a> <a id="905" href="foundation-core.identity-types.html#1807" class="InductiveConstructor">refl</a> <a id="910" class="Symbol">=</a> <a id="912" href="foundation-core.equivalences.html#2481" class="Function">id-equiv</a>

<a id="UNIVALENCE"></a><a id="922" href="foundation-core.univalence.html#922" class="Function">UNIVALENCE</a> <a id="933" class="Symbol">:</a> <a id="935" class="Symbol">{</a><a id="936" href="foundation-core.univalence.html#936" class="Bound">i</a> <a id="938" class="Symbol">:</a> <a id="940" href="Agda.Primitive.html#597" class="Postulate">Level</a><a id="945" class="Symbol">}</a> <a id="947" class="Symbol">(</a><a id="948" href="foundation-core.univalence.html#948" class="Bound">A</a> <a id="950" href="foundation-core.univalence.html#950" class="Bound">B</a> <a id="952" class="Symbol">:</a> <a id="954" href="foundation-core.universe-levels.html#222" class="Primitive">UU</a> <a id="957" href="foundation-core.univalence.html#936" class="Bound">i</a><a id="958" class="Symbol">)</a> <a id="960" class="Symbol">→</a> <a id="962" href="foundation-core.universe-levels.html#222" class="Primitive">UU</a> <a id="965" class="Symbol">(</a><a id="966" href="Agda.Primitive.html#780" class="Primitive">lsuc</a> <a id="971" href="foundation-core.univalence.html#936" class="Bound">i</a><a id="972" class="Symbol">)</a>
<a id="974" href="foundation-core.univalence.html#922" class="Function">UNIVALENCE</a> <a id="985" href="foundation-core.univalence.html#985" class="Bound">A</a> <a id="987" href="foundation-core.univalence.html#987" class="Bound">B</a> <a id="989" class="Symbol">=</a> <a id="991" href="foundation-core.equivalences.html#1543" class="Function">is-equiv</a> <a id="1000" class="Symbol">(</a><a id="1001" href="foundation-core.univalence.html#833" class="Function">equiv-eq</a> <a id="1010" class="Symbol">{</a><a id="1011" class="Argument">A</a> <a id="1013" class="Symbol">=</a> <a id="1015" href="foundation-core.univalence.html#985" class="Bound">A</a><a id="1016" class="Symbol">}</a> <a id="1018" class="Symbol">{</a><a id="1019" class="Argument">B</a> <a id="1021" class="Symbol">=</a> <a id="1023" href="foundation-core.univalence.html#987" class="Bound">B</a><a id="1024" class="Symbol">})</a>
</pre>
## Properties

### The univalence axiom implies that the total space of equivalences is contractible

<pre class="Agda"><a id="1142" class="Keyword">abstract</a>
  <a id="is-contr-total-equiv-UNIVALENCE"></a><a id="1153" href="foundation-core.univalence.html#1153" class="Function">is-contr-total-equiv-UNIVALENCE</a> <a id="1185" class="Symbol">:</a> <a id="1187" class="Symbol">{</a><a id="1188" href="foundation-core.univalence.html#1188" class="Bound">i</a> <a id="1190" class="Symbol">:</a> <a id="1192" href="Agda.Primitive.html#597" class="Postulate">Level</a><a id="1197" class="Symbol">}</a> <a id="1199" class="Symbol">(</a><a id="1200" href="foundation-core.univalence.html#1200" class="Bound">A</a> <a id="1202" class="Symbol">:</a> <a id="1204" href="foundation-core.universe-levels.html#222" class="Primitive">UU</a> <a id="1207" href="foundation-core.univalence.html#1188" class="Bound">i</a><a id="1208" class="Symbol">)</a> <a id="1210" class="Symbol">→</a>
    <a id="1216" class="Symbol">((</a><a id="1218" href="foundation-core.univalence.html#1218" class="Bound">B</a> <a id="1220" class="Symbol">:</a> <a id="1222" href="foundation-core.universe-levels.html#222" class="Primitive">UU</a> <a id="1225" href="foundation-core.univalence.html#1188" class="Bound">i</a><a id="1226" class="Symbol">)</a> <a id="1228" class="Symbol">→</a> <a id="1230" href="foundation-core.univalence.html#922" class="Function">UNIVALENCE</a> <a id="1241" href="foundation-core.univalence.html#1200" class="Bound">A</a> <a id="1243" href="foundation-core.univalence.html#1218" class="Bound">B</a><a id="1244" class="Symbol">)</a> <a id="1246" class="Symbol">→</a> <a id="1248" href="foundation-core.contractible-types.html#993" class="Function">is-contr</a> <a id="1257" class="Symbol">(</a><a id="1258" href="foundation-core.dependent-pair-types.html#502" class="Record">Σ</a> <a id="1260" class="Symbol">(</a><a id="1261" href="foundation-core.universe-levels.html#222" class="Primitive">UU</a> <a id="1264" href="foundation-core.univalence.html#1188" class="Bound">i</a><a id="1265" class="Symbol">)</a> <a id="1267" class="Symbol">(λ</a> <a id="1270" href="foundation-core.univalence.html#1270" class="Bound">X</a> <a id="1272" class="Symbol">→</a> <a id="1274" href="foundation-core.univalence.html#1200" class="Bound">A</a> <a id="1276" href="foundation-core.equivalences.html#1608" class="Function Operator">≃</a> <a id="1278" href="foundation-core.univalence.html#1270" class="Bound">X</a><a id="1279" class="Symbol">))</a>
  <a id="1284" href="foundation-core.univalence.html#1153" class="Function">is-contr-total-equiv-UNIVALENCE</a> <a id="1316" href="foundation-core.univalence.html#1316" class="Bound">A</a> <a id="1318" href="foundation-core.univalence.html#1318" class="Bound">UA</a> <a id="1321" class="Symbol">=</a>
    <a id="1327" href="foundation-core.fundamental-theorem-of-identity-types.html#2162" class="Function">fundamental-theorem-id&#39;</a> <a id="1351" href="foundation-core.univalence.html#1316" class="Bound">A</a> <a id="1353" href="foundation-core.equivalences.html#2481" class="Function">id-equiv</a> <a id="1362" class="Symbol">(λ</a> <a id="1365" href="foundation-core.univalence.html#1365" class="Bound">B</a> <a id="1367" class="Symbol">→</a> <a id="1369" href="foundation-core.univalence.html#833" class="Function">equiv-eq</a><a id="1377" class="Symbol">)</a> <a id="1379" href="foundation-core.univalence.html#1318" class="Bound">UA</a>
</pre>
### Contractibility of the total space of equivalences implies univalence

<pre class="Agda"><a id="1470" class="Keyword">abstract</a>
  <a id="UNIVALENCE-is-contr-total-equiv"></a><a id="1481" href="foundation-core.univalence.html#1481" class="Function">UNIVALENCE-is-contr-total-equiv</a> <a id="1513" class="Symbol">:</a> <a id="1515" class="Symbol">{</a><a id="1516" href="foundation-core.univalence.html#1516" class="Bound">i</a> <a id="1518" class="Symbol">:</a> <a id="1520" href="Agda.Primitive.html#597" class="Postulate">Level</a><a id="1525" class="Symbol">}</a> <a id="1527" class="Symbol">(</a><a id="1528" href="foundation-core.univalence.html#1528" class="Bound">A</a> <a id="1530" class="Symbol">:</a> <a id="1532" href="foundation-core.universe-levels.html#222" class="Primitive">UU</a> <a id="1535" href="foundation-core.univalence.html#1516" class="Bound">i</a><a id="1536" class="Symbol">)</a> <a id="1538" class="Symbol">→</a>
    <a id="1544" href="foundation-core.contractible-types.html#993" class="Function">is-contr</a> <a id="1553" class="Symbol">(</a><a id="1554" href="foundation-core.dependent-pair-types.html#502" class="Record">Σ</a> <a id="1556" class="Symbol">(</a><a id="1557" href="foundation-core.universe-levels.html#222" class="Primitive">UU</a> <a id="1560" href="foundation-core.univalence.html#1516" class="Bound">i</a><a id="1561" class="Symbol">)</a> <a id="1563" class="Symbol">(λ</a> <a id="1566" href="foundation-core.univalence.html#1566" class="Bound">X</a> <a id="1568" class="Symbol">→</a> <a id="1570" href="foundation-core.univalence.html#1528" class="Bound">A</a> <a id="1572" href="foundation-core.equivalences.html#1608" class="Function Operator">≃</a> <a id="1574" href="foundation-core.univalence.html#1566" class="Bound">X</a><a id="1575" class="Symbol">))</a> <a id="1578" class="Symbol">→</a> <a id="1580" class="Symbol">(</a><a id="1581" href="foundation-core.univalence.html#1581" class="Bound">B</a> <a id="1583" class="Symbol">:</a> <a id="1585" href="foundation-core.universe-levels.html#222" class="Primitive">UU</a> <a id="1588" href="foundation-core.univalence.html#1516" class="Bound">i</a><a id="1589" class="Symbol">)</a> <a id="1591" class="Symbol">→</a> <a id="1593" href="foundation-core.univalence.html#922" class="Function">UNIVALENCE</a> <a id="1604" href="foundation-core.univalence.html#1528" class="Bound">A</a> <a id="1606" href="foundation-core.univalence.html#1581" class="Bound">B</a>
  <a id="1610" href="foundation-core.univalence.html#1481" class="Function">UNIVALENCE-is-contr-total-equiv</a> <a id="1642" href="foundation-core.univalence.html#1642" class="Bound">A</a> <a id="1644" href="foundation-core.univalence.html#1644" class="Bound">c</a> <a id="1646" class="Symbol">=</a>
    <a id="1652" href="foundation-core.fundamental-theorem-of-identity-types.html#1891" class="Function">fundamental-theorem-id</a> <a id="1675" href="foundation-core.univalence.html#1642" class="Bound">A</a> <a id="1677" href="foundation-core.equivalences.html#2481" class="Function">id-equiv</a> <a id="1686" href="foundation-core.univalence.html#1644" class="Bound">c</a> <a id="1688" class="Symbol">(λ</a> <a id="1691" href="foundation-core.univalence.html#1691" class="Bound">B</a> <a id="1693" class="Symbol">→</a> <a id="1695" href="foundation-core.univalence.html#833" class="Function">equiv-eq</a><a id="1703" class="Symbol">)</a>
</pre>
### Computing transport

<pre class="Agda"><a id="tr-equiv-eq-ap"></a><a id="1743" href="foundation-core.univalence.html#1743" class="Function">tr-equiv-eq-ap</a> <a id="1758" class="Symbol">:</a> <a id="1760" class="Symbol">{</a><a id="1761" href="foundation-core.univalence.html#1761" class="Bound">l1</a> <a id="1764" href="foundation-core.univalence.html#1764" class="Bound">l2</a> <a id="1767" class="Symbol">:</a> <a id="1769" href="Agda.Primitive.html#597" class="Postulate">Level</a><a id="1774" class="Symbol">}</a> <a id="1776" class="Symbol">{</a><a id="1777" href="foundation-core.univalence.html#1777" class="Bound">A</a> <a id="1779" class="Symbol">:</a> <a id="1781" href="foundation-core.universe-levels.html#222" class="Primitive">UU</a> <a id="1784" href="foundation-core.univalence.html#1761" class="Bound">l1</a><a id="1786" class="Symbol">}</a> <a id="1788" class="Symbol">{</a><a id="1789" href="foundation-core.univalence.html#1789" class="Bound">B</a> <a id="1791" class="Symbol">:</a> <a id="1793" href="foundation-core.univalence.html#1777" class="Bound">A</a> <a id="1795" class="Symbol">→</a> <a id="1797" href="foundation-core.universe-levels.html#222" class="Primitive">UU</a> <a id="1800" href="foundation-core.univalence.html#1764" class="Bound">l2</a><a id="1802" class="Symbol">}</a> <a id="1804" class="Symbol">{</a><a id="1805" href="foundation-core.univalence.html#1805" class="Bound">x</a> <a id="1807" href="foundation-core.univalence.html#1807" class="Bound">y</a> <a id="1809" class="Symbol">:</a> <a id="1811" href="foundation-core.univalence.html#1777" class="Bound">A</a><a id="1812" class="Symbol">}</a>
  <a id="1816" class="Symbol">(</a><a id="1817" href="foundation-core.univalence.html#1817" class="Bound">p</a> <a id="1819" class="Symbol">:</a> <a id="1821" href="foundation-core.univalence.html#1805" class="Bound">x</a> <a id="1823" href="foundation-core.identity-types.html#1852" class="Function Operator">＝</a> <a id="1825" href="foundation-core.univalence.html#1807" class="Bound">y</a><a id="1826" class="Symbol">)</a> <a id="1828" class="Symbol">→</a> <a id="1830" class="Symbol">(</a><a id="1831" href="foundation-core.equivalences.html#1808" class="Function">map-equiv</a> <a id="1841" class="Symbol">(</a><a id="1842" href="foundation-core.univalence.html#833" class="Function">equiv-eq</a> <a id="1851" class="Symbol">(</a><a id="1852" href="foundation-core.identity-types.html#3990" class="Function">ap</a> <a id="1855" href="foundation-core.univalence.html#1789" class="Bound">B</a> <a id="1857" href="foundation-core.univalence.html#1817" class="Bound">p</a><a id="1858" class="Symbol">)))</a> <a id="1862" href="foundation-core.homotopies.html#614" class="Function Operator">~</a> <a id="1864" href="foundation-core.identity-types.html#5689" class="Function">tr</a> <a id="1867" href="foundation-core.univalence.html#1789" class="Bound">B</a> <a id="1869" href="foundation-core.univalence.html#1817" class="Bound">p</a>
<a id="1871" href="foundation-core.univalence.html#1743" class="Function">tr-equiv-eq-ap</a> <a id="1886" href="foundation-core.identity-types.html#1807" class="InductiveConstructor">refl</a> <a id="1891" class="Symbol">=</a> <a id="1893" href="foundation-core.homotopies.html#728" class="Function">refl-htpy</a>
</pre>