---
title: Opposite rings
---

<pre class="Agda"><a id="40" class="Symbol">{-#</a> <a id="44" class="Keyword">OPTIONS</a> <a id="52" class="Pragma">--without-K</a> <a id="64" class="Pragma">--exact-split</a> <a id="78" class="Symbol">#-}</a>

<a id="83" class="Keyword">module</a> <a id="90" href="ring-theory.opposite-rings.html" class="Module">ring-theory.opposite-rings</a> <a id="117" class="Keyword">where</a>

<a id="124" class="Keyword">open</a> <a id="129" class="Keyword">import</a> <a id="136" href="foundation.dependent-pair-types.html" class="Module">foundation.dependent-pair-types</a>
<a id="168" class="Keyword">open</a> <a id="173" class="Keyword">import</a> <a id="180" href="foundation.identity-types.html" class="Module">foundation.identity-types</a>
<a id="206" class="Keyword">open</a> <a id="211" class="Keyword">import</a> <a id="218" href="foundation.universe-levels.html" class="Module">foundation.universe-levels</a>

<a id="246" class="Keyword">open</a> <a id="251" class="Keyword">import</a> <a id="258" href="ring-theory.rings.html" class="Module">ring-theory.rings</a>
</pre>
## Idea

The opposite of a ring R is a ring with the same underlying abelian group, but with multiplication given by `xÂ·y := yx`.

## Definition

<pre class="Agda"><a id="435" class="Keyword">module</a> <a id="442" href="ring-theory.opposite-rings.html#442" class="Module">_</a>
  <a id="446" class="Symbol">{</a><a id="447" href="ring-theory.opposite-rings.html#447" class="Bound">l</a> <a id="449" class="Symbol">:</a> <a id="451" href="Agda.Primitive.html#597" class="Postulate">Level</a><a id="456" class="Symbol">}</a> <a id="458" class="Symbol">(</a><a id="459" href="ring-theory.opposite-rings.html#459" class="Bound">R</a> <a id="461" class="Symbol">:</a> <a id="463" href="ring-theory.rings.html#2458" class="Function">Ring</a> <a id="468" href="ring-theory.opposite-rings.html#447" class="Bound">l</a><a id="469" class="Symbol">)</a>
  <a id="473" class="Keyword">where</a>

  <a id="482" href="ring-theory.opposite-rings.html#482" class="Function">op-Ring</a> <a id="490" class="Symbol">:</a> <a id="492" href="ring-theory.rings.html#2458" class="Function">Ring</a> <a id="497" href="ring-theory.opposite-rings.html#447" class="Bound">l</a>
  <a id="501" href="foundation-core.dependent-pair-types.html#592" class="Field">pr1</a> <a id="505" href="ring-theory.opposite-rings.html#482" class="Function">op-Ring</a> <a id="513" class="Symbol">=</a> <a id="515" href="ring-theory.rings.html#2572" class="Function">ab-Ring</a> <a id="523" href="ring-theory.opposite-rings.html#459" class="Bound">R</a>
  <a id="527" href="foundation-core.dependent-pair-types.html#592" class="Field">pr1</a> <a id="531" class="Symbol">(</a><a id="532" href="foundation-core.dependent-pair-types.html#592" class="Field">pr1</a> <a id="536" class="Symbol">(</a><a id="537" href="foundation-core.dependent-pair-types.html#604" class="Field">pr2</a> <a id="541" href="ring-theory.opposite-rings.html#482" class="Function">op-Ring</a><a id="548" class="Symbol">))</a> <a id="551" class="Symbol">=</a> <a id="553" href="ring-theory.rings.html#6529" class="Function">mul-Ring&#39;</a> <a id="563" href="ring-theory.opposite-rings.html#459" class="Bound">R</a>
  <a id="567" href="foundation-core.dependent-pair-types.html#604" class="Field">pr2</a> <a id="571" class="Symbol">(</a><a id="572" href="foundation-core.dependent-pair-types.html#592" class="Field">pr1</a> <a id="576" class="Symbol">(</a><a id="577" href="foundation-core.dependent-pair-types.html#604" class="Field">pr2</a> <a id="581" href="ring-theory.opposite-rings.html#482" class="Function">op-Ring</a><a id="588" class="Symbol">))</a> <a id="591" href="ring-theory.opposite-rings.html#591" class="Bound">x</a> <a id="593" href="ring-theory.opposite-rings.html#593" class="Bound">y</a> <a id="595" href="ring-theory.opposite-rings.html#595" class="Bound">z</a> <a id="597" class="Symbol">=</a> <a id="599" href="foundation-core.identity-types.html#1552" class="Function">inv</a> <a id="603" class="Symbol">(</a><a id="604" href="ring-theory.rings.html#6774" class="Function">associative-mul-Ring</a> <a id="625" href="ring-theory.opposite-rings.html#459" class="Bound">R</a> <a id="627" href="ring-theory.opposite-rings.html#595" class="Bound">z</a> <a id="629" href="ring-theory.opposite-rings.html#593" class="Bound">y</a> <a id="631" href="ring-theory.opposite-rings.html#591" class="Bound">x</a> <a id="633" class="Symbol">)</a>
  <a id="637" href="foundation-core.dependent-pair-types.html#592" class="Field">pr1</a> <a id="641" class="Symbol">(</a><a id="642" href="foundation-core.dependent-pair-types.html#592" class="Field">pr1</a> <a id="646" class="Symbol">(</a><a id="647" href="foundation-core.dependent-pair-types.html#604" class="Field">pr2</a> <a id="651" class="Symbol">(</a><a id="652" href="foundation-core.dependent-pair-types.html#604" class="Field">pr2</a> <a id="656" href="ring-theory.opposite-rings.html#482" class="Function">op-Ring</a><a id="663" class="Symbol">)))</a> <a id="667" class="Symbol">=</a> <a id="669" href="ring-theory.rings.html#7884" class="Function">one-Ring</a> <a id="678" href="ring-theory.opposite-rings.html#459" class="Bound">R</a>
  <a id="682" href="foundation-core.dependent-pair-types.html#592" class="Field">pr1</a> <a id="686" class="Symbol">(</a><a id="687" href="foundation-core.dependent-pair-types.html#604" class="Field">pr2</a> <a id="691" class="Symbol">(</a><a id="692" href="foundation-core.dependent-pair-types.html#592" class="Field">pr1</a> <a id="696" class="Symbol">(</a><a id="697" href="foundation-core.dependent-pair-types.html#604" class="Field">pr2</a> <a id="701" class="Symbol">(</a><a id="702" href="foundation-core.dependent-pair-types.html#604" class="Field">pr2</a> <a id="706" href="ring-theory.opposite-rings.html#482" class="Function">op-Ring</a><a id="713" class="Symbol">))))</a> <a id="718" class="Symbol">=</a> <a id="720" href="ring-theory.rings.html#8114" class="Function">right-unit-law-mul-Ring</a> <a id="744" href="ring-theory.opposite-rings.html#459" class="Bound">R</a>
  <a id="748" href="foundation-core.dependent-pair-types.html#604" class="Field">pr2</a> <a id="752" class="Symbol">(</a><a id="753" href="foundation-core.dependent-pair-types.html#604" class="Field">pr2</a> <a id="757" class="Symbol">(</a><a id="758" href="foundation-core.dependent-pair-types.html#592" class="Field">pr1</a> <a id="762" class="Symbol">(</a><a id="763" href="foundation-core.dependent-pair-types.html#604" class="Field">pr2</a> <a id="767" class="Symbol">(</a><a id="768" href="foundation-core.dependent-pair-types.html#604" class="Field">pr2</a> <a id="772" href="ring-theory.opposite-rings.html#482" class="Function">op-Ring</a><a id="779" class="Symbol">))))</a> <a id="784" class="Symbol">=</a> <a id="786" href="ring-theory.rings.html#7962" class="Function">left-unit-law-mul-Ring</a> <a id="809" href="ring-theory.opposite-rings.html#459" class="Bound">R</a>
  <a id="813" href="foundation-core.dependent-pair-types.html#592" class="Field">pr1</a> <a id="817" class="Symbol">(</a><a id="818" href="foundation-core.dependent-pair-types.html#604" class="Field">pr2</a> <a id="822" class="Symbol">(</a><a id="823" href="foundation-core.dependent-pair-types.html#604" class="Field">pr2</a> <a id="827" class="Symbol">(</a><a id="828" href="foundation-core.dependent-pair-types.html#604" class="Field">pr2</a> <a id="832" href="ring-theory.opposite-rings.html#482" class="Function">op-Ring</a><a id="839" class="Symbol">)))</a> <a id="843" href="ring-theory.opposite-rings.html#843" class="Bound">x</a> <a id="845" href="ring-theory.opposite-rings.html#845" class="Bound">y</a> <a id="847" href="ring-theory.opposite-rings.html#847" class="Bound">z</a> <a id="849" class="Symbol">=</a> <a id="851" href="ring-theory.rings.html#7313" class="Function">right-distributive-mul-add-Ring</a> <a id="883" href="ring-theory.opposite-rings.html#459" class="Bound">R</a> <a id="885" href="ring-theory.opposite-rings.html#845" class="Bound">y</a> <a id="887" href="ring-theory.opposite-rings.html#847" class="Bound">z</a> <a id="889" href="ring-theory.opposite-rings.html#843" class="Bound">x</a>
  <a id="893" href="foundation-core.dependent-pair-types.html#604" class="Field">pr2</a> <a id="897" class="Symbol">(</a><a id="898" href="foundation-core.dependent-pair-types.html#604" class="Field">pr2</a> <a id="902" class="Symbol">(</a><a id="903" href="foundation-core.dependent-pair-types.html#604" class="Field">pr2</a> <a id="907" class="Symbol">(</a><a id="908" href="foundation-core.dependent-pair-types.html#604" class="Field">pr2</a> <a id="912" href="ring-theory.opposite-rings.html#482" class="Function">op-Ring</a><a id="919" class="Symbol">)))</a> <a id="923" href="ring-theory.opposite-rings.html#923" class="Bound">x</a> <a id="925" href="ring-theory.opposite-rings.html#925" class="Bound">y</a> <a id="927" href="ring-theory.opposite-rings.html#927" class="Bound">z</a> <a id="929" class="Symbol">=</a> <a id="931" href="ring-theory.rings.html#7106" class="Function">left-distributive-mul-add-Ring</a> <a id="962" href="ring-theory.opposite-rings.html#459" class="Bound">R</a> <a id="964" href="ring-theory.opposite-rings.html#927" class="Bound">z</a> <a id="966" href="ring-theory.opposite-rings.html#923" class="Bound">x</a> <a id="968" href="ring-theory.opposite-rings.html#925" class="Bound">y</a>
</pre>